Foundation/Modal/Kripke/Hilbert/GrzDot3.lean
@@ -46,10 +46,42 @@ end Kripke
 
 namespace Hilbert.GrzDot3
 
+open Kripke.Grz
+
 instance Kripke.sound : Sound (Hilbert.GrzDot3) (Kripke.ReflexiveTransitiveAntiSymmetricConnectedFiniteFrameClass) := inferInstance
 
 instance Kripke.consistent : Entailment.Consistent (Hilbert.GrzDot3) :=
   Kripke.Hilbert.consistent_of_FiniteFrameClass ReflexiveTransitiveAntiSymmetricConnectedFiniteFrameClass
+
+instance complete : Complete (Hilbert.GrzDot3) (Kripke.ReflexiveTransitiveAntiSymmetricConnectedFiniteFrameClass) :=
+  complete_of_mem_miniCanonicalFrame Kripke.ReflexiveTransitiveAntiSymmetricConnectedFiniteFrameClass $ by
+    intro φ;
+    refine ⟨miniCanonicalFrame.reflexive, miniCanonicalFrame.transitive, miniCanonicalFrame.antisymm, ?_⟩;
+    intro x y z ⟨⟨Rxy₁, Rxy₂⟩, ⟨Rxz₁, Rxz₂⟩⟩;
+    apply or_iff_not_imp_left.mpr;
+    intro nRyz;
+    rcases (not_and_or.mp nRyz) with (nRyz | nRyz);
+    . push_neg at nRyz;
+      obtain ⟨ψ, hψ, ⟨hψy, hψz⟩⟩ := nRyz;
+      constructor;
+      . intro ξ hξ₁ hξ₂;
+        apply Rxy₁;
+        . exact hξ₁;
+        . sorry;
+      . intro hyz;
+        have exy := Rxy₂ ?_;
+        have exz := Rxz₂ ?_;
+        tauto;
+        . subst exy;
+          intro ξ hξ hξz;
+          sorry;
+        . intro ξ hξ hξy;
+          sorry;
+    . push_neg at nRyz;
+      replace ⟨nRyz₁, nRyz₂⟩ := nRyz;
+      constructor;
+      . sorry;
+      . sorry;
 
 end Hilbert.GrzDot3
 
